

34. Area Between Curves.

Consider the region bounded by $f(x) = \frac{x}{3}$ (a straight line through the origin) and $g(x) = \sqrt{x}$ (a parabola opening to the right).

- (a) **Sketching and Intersection Points:** First, find where the curves intersect by setting $f(x) = g(x)$:

$$\frac{x}{3} = \sqrt{x} \implies \frac{x^2}{9} = x \implies x^2 - 9x = 0 \implies x(x - 9) = 0$$

The intersection points are at $x = 0$ (where $y = 0$) and $x = 9$ (where $y = 3$). On the interval $(0, 9)$, test a point like $x = 1$: $g(1) = 1$ and $f(1) = 1/3$. Since $1 > 1/3$, the curve $g(x) = \sqrt{x}$ is on top.

- (b) **Vertical Slices (Δx):** When using vertical slices, we integrate with respect to x . The height of a slice is the upper function minus the lower function: Height = $g(x) - f(x)$. The width is Δx (or dx). The bounds are from $x = 0$ to $x = 9$.

$$\text{Area} = \int_0^9 \left(\sqrt{x} - \frac{x}{3} \right) dx$$

(Evaluation not required for this part).

- (c) **Horizontal Slices (Δy):** When using horizontal slices, we integrate with respect to y . We must express the functions as x in terms of y .

- $y = \frac{x}{3} \implies x = 3y$ (This is the line on the right).
- $y = \sqrt{x} \implies x = y^2$ (This is the parabola on the left).

The width of a slice is the right function minus the left function: Width = $3y - y^2$. The thickness is Δy (or dy). The bounds are from $y = 0$ to $y = 3$.

$$\text{Area} = \int_0^3 (3y - y^2) dy$$

(Evaluation not required for this part).

35. Integration by Parts.

Evaluate $\int x e^{-4x} dx$.

Step 1: Choose parts. Use the formula $\int u dv = uv - \int v du$. Choose u to be the part that gets simpler when differentiated, and dv to be the part that is easy to integrate.

- Let $u = x \implies du = dx$
- Let $dv = e^{-4x} dx \implies v = \int e^{-4x} dx = -\frac{1}{4}e^{-4x}$

Step 2: Apply formula.

$$\begin{aligned} \int x e^{-4x} dx &= (x) \left(-\frac{1}{4} e^{-4x} \right) - \int \left(-\frac{1}{4} e^{-4x} \right) dx \\ &= -\frac{1}{4} x e^{-4x} + \frac{1}{4} \int e^{-4x} dx \end{aligned}$$

Step 3: Evaluate the remaining integral.

$$= -\frac{1}{4}xe^{-4x} + \frac{1}{4}\left(-\frac{1}{4}e^{-4x}\right) + C$$

$$\boxed{-\frac{1}{4}xe^{-4x} - \frac{1}{16}e^{-4x} + C}$$

Step 4: Verification (Differentiation). Differentiate the result to check:

$$\frac{d}{dx} \left[-\frac{1}{4}xe^{-4x} - \frac{1}{16}e^{-4x} \right]$$

Using Product Rule on the first term:

$$\begin{aligned} & \left[-\frac{1}{4}(1)e^{-4x} + \left(-\frac{1}{4}x\right)(-4e^{-4x}) \right] - \frac{1}{16}(-4e^{-4x}) \\ &= -\frac{1}{4}e^{-4x} + xe^{-4x} + \frac{1}{4}e^{-4x} \\ &= xe^{-4x} \quad (\text{Correct}) \end{aligned}$$

36. Splitting Fractions Standard Integrals.

Evaluate $\int \frac{2+x}{1+x^2} dx$.

Step 1: Split the numerator. Separate the integral into two simpler parts:

$$I = \int \frac{2}{1+x^2} dx + \int \frac{x}{1+x^2} dx$$

Step 2: Evaluate the first part. Recognize that $\int \frac{1}{1+x^2} dx = \arctan(x)$.

$$\int \frac{2}{1+x^2} dx = 2 \arctan(x)$$

Step 3: Evaluate the second part. Use substitution for $\int \frac{x}{1+x^2} dx$. Let $w = 1 + x^2$, then $dw = 2x dx \implies x dx = \frac{1}{2} dw$.

$$\int \frac{1}{w} \cdot \frac{1}{2} dw = \frac{1}{2} \ln|w| = \frac{1}{2} \ln(1+x^2)$$

(Note: $1+x^2$ is always positive, so absolute value bars are optional).

Step 4: Combine.

$$\boxed{2 \arctan(x) + \frac{1}{2} \ln(1+x^2) + C}$$

37. Mixed Integration Techniques.

(a) **Evaluate** $\int x e^{-3x^2} dx$.

Method: Substitution. Let $w = -3x^2$. Then $\frac{dw}{dx} = -6x \implies x dx = -\frac{1}{6} dw$.

Substitute into the integral:

$$\begin{aligned} \int e^w \left(-\frac{1}{6}\right) dw &= -\frac{1}{6} \int e^w dw \\ &= -\frac{1}{6} e^w + C \end{aligned}$$

Substitute back $w = -3x^2$:

$$\boxed{-\frac{1}{6} e^{-3x^2} + C}$$

(b) **Evaluate** $\int \arccos(x) dx$.

Method: Integration by Parts. Let $u = \arccos(x)$ and $dv = dx$.

- $du = -\frac{1}{\sqrt{1-x^2}} dx$
- $v = x$

Apply formula:

$$\begin{aligned} I &= x \arccos(x) - \int x \left(-\frac{1}{\sqrt{1-x^2}}\right) dx \\ I &= x \arccos(x) + \int \frac{x}{\sqrt{1-x^2}} dx \end{aligned}$$

Now, use substitution for the remaining integral. Let $w = 1 - x^2$, then $dw = -2x dx \implies x dx = -\frac{1}{2} dw$.

$$\begin{aligned} \int w^{-1/2} \left(-\frac{1}{2}\right) dw &= -\frac{1}{2} \int w^{-1/2} dw \\ &= -\frac{1}{2} (2w^{1/2}) = -\sqrt{w} = -\sqrt{1-x^2} \end{aligned}$$

Combine with the first part:

$$\boxed{x \arccos(x) - \sqrt{1-x^2} + C}$$